Values.thy
@@ -7,11 +7,6 @@ begin
 
 type_synonym objref = "nat option"
 
-datatype UnstampedValue =
-  UnstampedFloat (uv_m: int) (uv_e: int) |
-  UnstampedInt (uv_i: int) |
-  UnstampedObj (uv_n: objref)
-
 datatype Value  =
   UndefVal |
   IntVal (v_bits: int) (v_int: int) |
